prove heap alloc and free

ex/FailureEx.thy
@@ -3,145 +3,156 @@ theory FailureEx
 begin
 
 (* TODO: move *)
+lemma comp_inf_distrib:
+  \<open>(a \<sqinter> b) \<circ> f = (a \<circ> f) \<sqinter> (b \<circ> f)\<close>
+  by force
+
+lemma comp_sup_distrib:
+  \<open>(a \<squnion> b) \<circ> f = (a \<circ> f) \<squnion> (b \<circ> f)\<close>
+  by force
+
 lemma option_ex_split:
   \<open>(case mx of Some x \<Rightarrow> p x | None \<Rightarrow> q) \<longleftrightarrow> (\<exists>x. mx = Some x \<and> p x) \<or> mx = None \<and> q\<close>
   by (metis case_option_disj_iff)
+
+
+section \<open> Helper Lemmas \<close>
+
+subsection \<open> Heap Lemmas \<close>
+
+lemma heap_upd_eq_iff:
+  \<open>ha(x \<mapsto>  va) = hb(x \<mapsto>  vb) \<longleftrightarrow> (\<forall>y. y \<noteq> x \<longrightarrow> ha y = hb y) \<and> va = vb\<close>
+  by (force simp add: fun_eq_iff)
+
+lemma not_dom_then_singleton_plus_heap_eq[simp]:
+  \<open>h x = None \<Longrightarrow> [x \<mapsto> v] + h = h(x \<mapsto> v)\<close>
+  by (simp add: fun_eq_iff)
+
+lemma map_empty_disjoint[simp]:
+  \<open>Map.empty ## mb\<close>
+  \<open>ma ## Map.empty\<close>
+  by (simp add: disjoint_fun_def)+
+
+lemma map_empty_plus[simp]:
+  \<open>Map.empty + mb = mb\<close>
+  \<open>ma + Map.empty = ma\<close>
+  by (simp add: fun_eq_iff)+
 
 lemma singleton_plus_heap_eq_iff:
   \<open>[x \<mapsto> va] + h = [x \<mapsto> vb] + h \<longleftrightarrow> Some va + h x = Some vb + h x\<close>
   by (simp add: plus_fun_def plus_option_def fun_eq_iff split: option.splits if_splits)
 
+lemma heap_upd_eq_singleton_plus_heap_iff:
+  \<open>hx(x \<mapsto>  va) = [x \<mapsto> vb] + hy \<longleftrightarrow> (\<forall>y. y \<noteq> x \<longrightarrow> hx y = hy y) \<and> Some vb + hy x = Some va\<close>
+  by (force simp add: plus_fun_def plus_option_def fun_eq_iff split: option.splits if_splits)
 
 
-subsection \<open> Heap predicate \<close>
+subsection \<open> Tuple rearrangement \<close>
 
-definition points_to :: \<open>'a \<Rightarrow> 'b \<Rightarrow> ('a \<rightharpoonup> 'b) \<Rightarrow> bool\<close> (infix \<open>\<^bold>\<mapsto>\<close> 90) where
-  \<open>p \<^bold>\<mapsto> x \<equiv> \<lambda>h. h p = Some x \<and> (\<forall>p'. p' \<noteq> p \<longrightarrow> h p' = None)\<close>
+definition \<open>pApBC_to_ppABC \<equiv> \<lambda>(a,(b,c)). ((a,b),c)\<close>
 
-definition points_to_upcl :: \<open>'a \<Rightarrow> 'b \<Rightarrow> ('a \<rightharpoonup> 'b) \<Rightarrow> bool\<close> (infix \<open>\<^bold>\<mapsto>\<^sup>\<Up>\<close> 90) where
-  \<open>p \<^bold>\<mapsto>\<^sup>\<Up> x \<equiv> \<lambda>h. h p = Some x\<close>
+lemma pApBC_to_ppACB_apply[simp]:
+  \<open>pApBC_to_ppABC (a,b,c) = ((a,b),c)\<close>
+  by (simp add: pApBC_to_ppABC_def split: prod.splits)
 
-abbreviation points_to_perm
-  :: \<open>'a \<Rightarrow> 'perm \<Rightarrow> 'b \<Rightarrow> ('a \<rightharpoonup> 'b discr \<times> 'perm) \<Rightarrow> bool\<close>
-  (\<open>_ \<^bold>\<mapsto>\<^bsub>_\<^esub> _\<close> [90,0,90] 90)
-  where
-  \<open>p \<^bold>\<mapsto>\<^bsub>perm\<^esub> v \<equiv> p \<^bold>\<mapsto> (Discr v, perm)\<close>
+lemma pApBC_to_ppACB_inj:
+  \<open>inj pApBC_to_ppABC\<close>
+  by (simp add: pApBC_to_ppABC_def inj_def split: prod.splits)
 
-lemma points_to_upcl_eq:
-  fixes x :: \<open>'a :: perm_alg\<close>
-  assumes maxsep_x: \<open>\<forall>x'. \<not> x ## x'\<close>
-  shows \<open>pt \<^bold>\<mapsto>\<^sup>\<Up> x = \<top> \<^emph> pt \<^bold>\<mapsto> x\<close>
-  unfolding sepconj_def points_to_def points_to_upcl_def
-  apply (clarsimp simp add: fun_eq_iff)
-  apply (rename_tac h)
-  apply (intro iffI)
-   apply (rule_tac x=\<open>h(pt := None)\<close> in exI)
-   apply (rule_tac x=\<open>[pt \<mapsto> x]\<close> in exI)
-   apply force
-  apply (clarsimp simp add: disjoint_option_def split: option.splits)
-  apply (clarsimp simp add: plus_option_iff)
-  apply (metis disjoint_fun_def disjoint_option_iff(1) disjoint_sym_iff maxsep_x)
+
+definition \<open>ppABC_to_ppACB \<equiv> \<lambda>((a,b),c). ((a,c),b)\<close>
+
+lemma ppABC_to_ppACB_apply[simp]:
+  \<open>ppABC_to_ppACB ((a,b),c) = ((a,c),b)\<close>
+  by (simp add: ppABC_to_ppACB_def split: prod.splits)
+
+lemma ppABC_to_ppACB_inj:
+  \<open>inj ppABC_to_ppACB\<close>
+  by (simp add: ppABC_to_ppACB_def inj_def split: prod.splits)
+
+lemma pred_times_ppABC_to_ppACB_local_left_eq[simp]:
+  \<open>(\<L> p \<times>\<^sub>P q \<circ> ppABC_to_ppACB) = \<L> (p \<times>\<^sub>P q)\<close>
+  by (simp add: fun_eq_iff sepconj_conj_def)
+
+lemma subpred_pred_times_eq_res_ppABC_to_ppACB_iff:
+  \<open>f \<le> (F \<times>\<^sub>P (=) x) \<circ> ppABC_to_ppACB \<longleftrightarrow> (\<exists>f'. f' \<le> F \<and> f = (f' \<times>\<^sub>P (=) x) \<circ> ppABC_to_ppACB)\<close>
+  apply (clarsimp simp add: le_fun_def fun_eq_iff)
+  apply (rule iffI)
+   apply (rule_tac x=\<open>\<lambda>(ls, ss). f ((ls, x), ss)\<close> in exI, force)
+  apply force
   done
 
+lemma all_subpred_pred_times_eq_res_ppABC_to_ppACB_internalise:
+  \<open>(\<forall>p\<le>(P \<times>\<^sub>P (=) x) \<circ> ppABC_to_ppACB. \<Q> p) \<longleftrightarrow> (\<forall>p\<le>P. \<Q> ((p \<times>\<^sub>P (=) x) \<circ> ppABC_to_ppACB))\<close>
+  by (clarsimp simp add: subpred_pred_times_eq_res_ppABC_to_ppACB_iff, blast)
 
-subsection \<open> Failure and Programs \<close>
+lemma pred_times_comp_ppABC_to_ppACB_eq[simp]:
+  \<open>(pa \<times>\<^sub>P pb) \<times>\<^sub>P pc \<circ> ppABC_to_ppACB = (pa \<times>\<^sub>P pc) \<times>\<^sub>P pb\<close>
+  by force
 
-text \<open> Failure should not be resolvable. \<close>
-definition
-  \<open>step_fail_lift ra \<equiv>
-    (\<lambda>(ls, (ss, fl)) s'.
-        fl = Running \<and> ra (ls, ss) s' \<or>
-        fl = Failed \<and> s' = (ls, ss, fl))\<close>
+lemma pred_image_fst_pred_times_eq_res_ppABC_to_ppACB_eq[simp]:
+  \<open>pred_image fst ((p \<times>\<^sub>P q) \<circ> ppABC_to_ppACB) = pred_image fst p \<times>\<^sub>P q\<close>
+  by (clarsimp simp add: fun_eq_iff)
 
-lemma failure_healthy_rel_apply[simp]:
-  \<open>step_fail_lift ra s s' =
-    (snd (snd s) = Running \<and> ra (fst s, fst (snd s)) s' \<or>
-     snd (snd s) = Failed \<and> s' = s)\<close>
-  by (simp add: step_fail_lift_def prod_eq_iff split: prod.splits)
+lemma any_shared_pred_times_eq_res_ppABC_to_ppACB_distrib:
+  \<open>any_shared ((p \<times>\<^sub>P q) \<circ> ppABC_to_ppACB) = (any_shared p \<times>\<^sub>P q) \<circ> ppABC_to_ppACB\<close>
+  by (simp add: any_shared_def)
 
 
-subsection \<open> Failure definitions \<close>
+\<comment> \<open> any_shared if of this form \<close>
+lemma pred_image_fst_pred_times_eq_res_ppABC_to_ppACB_distrib:
+  \<open>pred_image fst ((p \<times>\<^sub>P q) \<circ> ppABC_to_ppACB) \<times>\<^sub>P qy =
+    ((pred_image fst p \<times>\<^sub>P qy) \<times>\<^sub>P q) \<circ> ppABC_to_ppACB\<close>
+  by (force simp add: fun_eq_iff)
 
-definition pred_Times_third
-  :: \<open>('a \<times> 'b \<Rightarrow> bool) \<Rightarrow> ('c \<Rightarrow> bool) \<Rightarrow> ('a \<times> ('b \<times> 'c) \<Rightarrow> bool)\<close>
-  (infix \<open>\<times>\<^sub>P\<^sub>3\<close> 80)
+lemma comp_ppABC_to_ppACB_mono[intro]:
+  \<open>pa \<le> pb \<Longrightarrow> pa \<circ> ppABC_to_ppACB \<le> pb \<circ> ppABC_to_ppACB\<close>
+  by (clarsimp simp add: le_fun_def)
+
+
+subsection \<open> X \<close>
+
+\<comment> \<open> A 'local' predicate that may depend on the shared state. \<close>
+abbreviation(input) local_pred_with_shared
+  :: \<open>('b \<Rightarrow> 'a \<Rightarrow> bool) \<Rightarrow> ('a \<times> 'b \<Rightarrow> bool)\<close> (\<open>\<L>\<^sub>S\<close>)
   where
-  \<open>p \<times>\<^sub>P\<^sub>3 q \<equiv> \<lambda>(a,(b,c)). p (a,b) \<and> q c\<close>
-
-lemma pred_Times_third_apply[simp]:
-  \<open>(p \<times>\<^sub>P\<^sub>3 q) x = (p (fst x, fst (snd x)) \<and> q (snd (snd x)))\<close>
-  by (simp add: pred_Times_third_def split: prod.splits)
+    \<open>\<L>\<^sub>S p \<equiv> \<lambda>(ls, ss). p ss ls\<close>
 
 
-abbreviation
-  \<open>nofailure_pred p \<equiv> p \<times>\<^sub>P\<^sub>3 (=) Running\<close>
 
-lemmas nofailure_pred_def =
-  pred_Times_third_def[of _ \<open>(=) Running\<close>]
+subsection \<open> Failure \<close>
+
+subsection \<open> Definitions \<close>
 
 abbreviation
-  \<open>failure_pred p \<equiv> p \<times>\<^sub>P\<^sub>3 (=) Failed\<close>
+  \<open>nofailure_pred p \<equiv> (p \<times>\<^sub>P (=) Running) \<circ> ppABC_to_ppACB\<close>
 
-lemmas failure_pred_def =
-  pred_Times_third_def[of _ \<open>(=) Running\<close>]
+abbreviation
+  \<open>failure_pred p \<equiv> (p \<times>\<^sub>P (=) Failed) \<circ> ppABC_to_ppACB\<close>
+
+lemma nofailure_pred_strong_mono[simp]:
+  \<open>nofailure_pred p \<le> nofailure_pred q \<longleftrightarrow> p \<le> q\<close>
+  by (simp add: le_fun_def)
+
+\<comment> \<open> These two only work because the fail_st resources are duplicable, i.e. \<open>a + a = a\<close>. \<close>
+lemma nofailure_pred_sepconj_conj_distrib:
+  \<open>nofailure_pred (pa \<^emph>\<and> pb) = nofailure_pred pa \<^emph>\<and> nofailure_pred pb\<close>
+  using plus_fail_st_def
+  by (force simp add: fun_eq_iff sepconj_conj_def)
+
+lemma failure_pred_sepconj_conj_distrib:
+  \<open>failure_pred (pa \<^emph>\<and> pb) = failure_pred pa \<^emph>\<and> failure_pred pb\<close>
+  using plus_fail_st_def
+  by (force simp add: fun_eq_iff sepconj_conj_def)
+
 
 abbreviation failure_rgsat_pretty
   (\<open>_, _, _, _, _ \<turnstile>\<^sub>f { _ } _ { _ }\<close> [55, 0, 0, 0, 0, 55, 55, 55] 56) where
   \<open>R, G, I, F, T \<turnstile>\<^sub>f { p } c { q } \<equiv>
-    rgsat c
-      (R \<times>\<^sub>R (=)) (G \<times>\<^sub>R (=))
+    rgsat c R G
       (nofailure_pred p) (nofailure_pred q)
       (nofailure_pred I) (nofailure_pred F)
       T\<close>
-
-
-lemma predTimes3_sepconj_conj_distrib:
-  \<open>(p \<^emph>\<and> f) \<times>\<^sub>P\<^sub>3 q = p \<times>\<^sub>P\<^sub>3 q \<^emph>\<and> f \<times>\<^sub>P\<^sub>3 q\<close>
-  by (force simp add: pred_Times_third_def sepconj_conj_apply fun_eq_iff)
-
-lemma predTimes3_inf_distrib:
-  \<open>(p \<sqinter> f) \<times>\<^sub>P\<^sub>3 q = p \<times>\<^sub>P\<^sub>3 q \<sqinter> f \<times>\<^sub>P\<^sub>3 q\<close>
-  by (force simp add: pred_Times_third_def sepconj_conj_apply fun_eq_iff)
-
-lemma predTimes3_sup_distrib:
-  \<open>(p \<squnion> f) \<times>\<^sub>P\<^sub>3 q = p \<times>\<^sub>P\<^sub>3 q \<squnion> f \<times>\<^sub>P\<^sub>3 q\<close>
-  by (force simp add: pred_Times_third_def sepconj_conj_apply fun_eq_iff)
-
-
-lemma sp_triple_relTimes_predTimes3_eq[simp]:
-  \<open>sp (ra \<times>\<^sub>R (rb \<times>\<^sub>R rc)) (p \<times>\<^sub>P\<^sub>3 q) = sp (ra \<times>\<^sub>R rb) p \<times>\<^sub>P\<^sub>3 sp rc q\<close>
-  by (force simp add: sp_def pred_Times_third_def)
-
-lemma reflp_wlp_equals_predTimes3_eq[simp]:
-  \<open>reflp ra \<Longrightarrow> reflp rb \<Longrightarrow>
-    wlp (ra \<times>\<^sub>R rb \<times>\<^sub>R (=)) (p \<times>\<^sub>P\<^sub>3 q) = wlp (ra \<times>\<^sub>R rb) p \<times>\<^sub>P\<^sub>3 q\<close>
-  by (force simp add: wlp_def pred_Times_third_def fun_eq_iff reflp_def)
-
-lemma predTimes3_eqVal_le_iff[simp]:
-  \<open>pa \<times>\<^sub>P\<^sub>3 (=) v \<le> pb \<times>\<^sub>P\<^sub>3 (=) v \<longleftrightarrow> pa \<le> pb\<close>
-  by (force simp add: pred_Times_third_def)
-
-lemma subset_nofailure_pred_iff:
-  \<open>f \<le> nofailure_pred F \<longleftrightarrow> (\<exists>f'. f' \<le> F \<and> f = nofailure_pred f')\<close>
-  apply (clarsimp simp add: nofailure_pred_def le_fun_def fun_eq_iff)
-  apply (rule iffI)
-   apply (rule_tac x=\<open>\<lambda>(ls, ss). f (ls, ss, Running)\<close> in exI, force)
-  apply force
-  done
-
-lemma all_impl_nofailure_pred_internalise:
-  \<open>(\<forall>p\<le>nofailure_pred P. q p) \<longleftrightarrow> (\<forall>p\<le>P. q (nofailure_pred p))\<close>
-  by (simp add: subset_nofailure_pred_iff, metis)
-
-lemma sp_step_fail_lift_on_nofailure_pred_eq:
-  \<open>sp (step_fail_lift r) (nofailure_pred p) =
-    (\<lambda>(l', s', k'). (\<exists>s. r s (l', s', k') \<and> p s))\<close>
-  by (simp add: sp_def fun_eq_iff)
-
-lemma nofailure_local_eq:
-  \<open>nofailure_pred (\<L> p) = \<L> p \<sqinter> nofailure_pred \<top>\<close>
-  unfolding nofailure_pred_def
-  by (simp add: fun_eq_iff sepconj_conj_def)
 
 
 section \<open> Assert \<close>
@@ -153,49 +164,38 @@ text \<open>
   and, moreover, atoms see the whole state, not the local state.
   Thus we place a crash in the shared state.
 \<close>
-definition \<open>Assert p \<equiv>
-  Atomic (step_fail_lift (\<lambda>(l, s) (l', s', fl').
-    l' = l \<and> s' = s \<and> (p (l, s) \<and> fl' = Running \<or> \<not> p (l, s) \<and> fl' = Failed)
-  ))\<close>
+definition
+  \<open>assert_rel p \<equiv> \<lambda>((l,fl),s) ((l',fl'),s').
+    l' = l \<and> s' = s \<and> (
+      p (l, s) \<and> fl = Running \<and> fl' = Running \<or> (\<not> p (l, s) \<or> fl = Failed) \<and> fl' = Failed)\<close>
+
+abbreviation \<open>Assert p \<equiv> \<langle> assert_rel p \<rangle>\<close>
+lemmas Assert_def = assert_rel_def
+
 
 lemma rgsat_assert:
-  assumes precond:
+  assumes
     \<open>p \<^emph>\<and> F \<le> pa\<close>
-    and guar:
     \<open>rel_image snd (rel_liftL (p \<^emph>\<and> F) \<sqinter> (=)) \<le> G\<close>
-    and inv:
     \<open>sswa R p \<le> I\<close>
-    and tree:
     \<open>T RGSepAtom\<close>
   shows
     \<open>R, G, I, F, T \<turnstile>\<^sub>f { wssa R p } Assert pa { sswa R p }\<close>
   using assms
-  unfolding Assert_def
 proof (intro rgsat_atom[where p=\<open>nofailure_pred p\<close> and q=\<open>nofailure_pred p\<close>])
-  let ?ra' = \<open>(step_fail_lift
-            (\<lambda>(l, s) (l', s', k').
-                l' = l \<and>
-                s' = s \<and> (pa (l, s) \<and> k' = Running \<or> \<not> pa (l, s) \<and> k' = Failed)))\<close>
-
   show
     \<open>\<forall>f\<le>nofailure_pred F.
-       sp ?ra' (nofailure_pred p \<^emph>\<and> f) \<le> nofailure_pred p \<^emph>\<and> any_shared f\<close>
-    using precond
-    by (simp add: all_impl_nofailure_pred_internalise
-        predTimes3_sepconj_conj_distrib[symmetric] sp_step_fail_lift_on_nofailure_pred_eq,
-        fastforce simp add: le_fun_def sepconj_conj_apply any_shared_def)
+      sp (assert_rel pa) (nofailure_pred p \<^emph>\<and> f) \<le> nofailure_pred p \<^emph>\<and> any_shared f\<close>
+    using assms(1)
+    apply (simp add: assert_rel_def all_subpred_pred_times_eq_res_ppABC_to_ppACB_internalise)
+    apply (clarsimp simp add: sp_def sepconj_conj_def)
+    apply blast
+    done
 
-  show
-    \<open>rel_image snd
-      (rel_liftL (nofailure_pred p \<^emph>\<and> nofailure_pred F) \<sqinter> ?ra')
-      \<le> G \<times>\<^sub>R (=)\<close>
-    using guar precond
-    by (force simp add: predTimes3_sepconj_conj_distrib[symmetric])
-
-  show \<open>sswa (R \<times>\<^sub>R (=)) (nofailure_pred p) \<le> nofailure_pred I\<close>
-    using assms
-    by force
-qed (simp add: sswa_weaker wssa_stronger)+
+  show \<open>rel_image snd (rel_liftL (nofailure_pred p \<^emph>\<and> nofailure_pred F) \<sqinter> assert_rel pa) \<le> G\<close>
+    using assms(2)
+    by (fastforce simp add: nofailure_pred_sepconj_conj_distrib[symmetric] assert_rel_def)
+qed (clarsimp simp add: wlp_def sp_def le_fun_def)+
 
 lemma frame_expanding_iff:
   \<open>(\<forall>f\<le>F. (p \<sqinter> pa) \<^emph>\<and> f \<le> (p \<^emph>\<and> any_shared f) \<sqinter> pa) \<longleftrightarrow>
@@ -214,274 +214,390 @@ lemma rgsat_assert2:
   by (blast intro: rgsat_assert)
 
 lemma opstep_assert_iff[simp]:
+  defines \<open>local \<equiv> fst \<circ> fst\<close>
+    and \<open>failst \<equiv> snd \<circ> fst\<close>
+    and \<open>shared \<equiv> snd\<close>
+  shows
   \<open>opstep \<alpha> (s, Assert p) sc' \<longleftrightarrow>
     \<alpha> = Vis \<and>
     snd sc' = Skip \<and>
-    (snd (snd s) = Running \<and>
-      fst (fst sc') = fst s \<and>
-      fst (snd (fst sc')) = fst (snd s) \<and>
-      (p (fst s, fst (snd s)) \<and> snd (snd (fst sc')) = Running \<or>
-        \<not> p (fst s, fst (snd s)) \<and> snd (snd (fst sc')) = Failed) \<or>
-      snd (snd s) = Failed \<and> s = fst sc')\<close>
-  by (force simp add: Assert_def case_prod_beta)
+    (local (fst sc') = local s \<and>
+      shared (fst sc') = shared s \<and>
+      (p (local s, shared s) \<and> failst s = Running \<and> failst (fst sc') = Running \<or>
+        (\<not> p (local s, shared s) \<or> failst s = Failed) \<and> failst (fst sc') = Failed))\<close>
+  using assms
+  by (force simp add: Assert_def case_prod_beta split_pairs2)
 
 
-section \<open> PointerRead \<close>
+section \<open> Heap Predicates \<close>
 
-definition PointerRead
-  :: \<open>'x \<Rightarrow> 'pt \<Rightarrow> (('pt \<rightharpoonup> 'v discr \<times> 'perm) \<times> (('x \<Rightarrow> 'v) \<times> fail_st)) comm\<close>
+definition points_to :: \<open>'a \<Rightarrow> 'b \<Rightarrow> ('a \<rightharpoonup> 'b) \<Rightarrow> bool\<close> (infix \<open>\<^bold>\<mapsto>\<close> 90) where
+  \<open>p \<^bold>\<mapsto> x \<equiv> \<lambda>h. h p = Some x \<and> (\<forall>p'. p' \<noteq> p \<longrightarrow> h p' = None)\<close>
+
+definition points_to_upcl :: \<open>'a \<Rightarrow> 'b \<Rightarrow> ('a \<rightharpoonup> 'b) \<Rightarrow> bool\<close> (infix \<open>\<^bold>\<mapsto>\<^sup>\<Up>\<close> 90) where
+  \<open>p \<^bold>\<mapsto>\<^sup>\<Up> x \<equiv> \<lambda>h. h p = Some x\<close>
+
+definition points_to_perm
+  :: \<open>'pt \<Rightarrow> 'perm \<Rightarrow> ('s \<Rightarrow> 'v) \<Rightarrow> ('pt \<rightharpoonup> 'v discr \<times> 'perm) \<times> 's \<Rightarrow> bool\<close>
+  (\<open>_ \<^bold>\<mapsto>\<^bsub>_\<^esub> _\<close> [90,0,90] 90)
   where
-    \<open>PointerRead x pt \<equiv>
-      Atomic (step_fail_lift (\<lambda>(l, s) (l', s', fl').
-        case l pt of
-          Some (v, _) \<Rightarrow> l' = l \<and> s' = s(x := the_discr v) \<and> fl' = Running
-        | None \<Rightarrow> l' = l \<and> s' = s \<and> fl' = Failed
-      ))\<close>
+  \<open>pt \<^bold>\<mapsto>\<^bsub>perm\<^esub> e \<equiv> \<lambda>(ls,ss). (=) [pt \<mapsto> (Discr (e ss), perm)] ls\<close>
 
-lemma rgsat_pointer_read:
-  fixes x v p R \<pi> pt
-  defines \<open>ra_ptr_read \<equiv> (=) \<times>\<^sub>R (\<lambda>s s'. s' = s(x := v))\<close>
-  and \<open>precond \<equiv> \<L> (pt \<^bold>\<mapsto>\<^bsub>\<pi>\<^esub> v) \<sqinter> wssa R (\<S> (\<lambda>s. p (s(x := v))))\<close>
-  and \<open>postcond \<equiv> \<L> (pt \<^bold>\<mapsto>\<^bsub>\<pi>\<^esub> v) \<sqinter> sswa R (\<S> p)\<close>
+lemma points_to_upcl_eq:
+  fixes x :: \<open>'a :: perm_alg\<close>
+  assumes maxsep_x: \<open>\<forall>x'. \<not> x ## x'\<close>
+  shows \<open>pt \<^bold>\<mapsto>\<^sup>\<Up> x = \<top> \<^emph> pt \<^bold>\<mapsto> x\<close>
+  unfolding sepconj_def points_to_def points_to_upcl_def
+  apply (clarsimp simp add: fun_eq_iff)
+  apply (rename_tac h)
+  apply (intro iffI)
+   apply (rule_tac x=\<open>h(pt := None)\<close> in exI)
+   apply (rule_tac x=\<open>[pt \<mapsto> x]\<close> in exI)
+   apply force
+  apply (clarsimp simp add: disjoint_option_def split: option.splits)
+  apply (clarsimp simp add: plus_option_iff)
+  apply (metis disjoint_fun_def disjoint_option_iff(1) disjoint_sym_iff maxsep_x)
+  done
+
+definition \<open>maximal_heap h \<equiv> \<forall>pt. h pt \<noteq> None\<close>
+
+abbreviation \<open>heap_pred p \<equiv> (p \<times>\<^sub>P \<top>) \<circ> ppABC_to_ppACB\<close>
+
+
+section \<open> Heap Commands \<close>
+
+subsection \<open> Heap Read \<close>
+
+definition heap_read_rel
+  :: \<open>'x \<Rightarrow> 'pt \<Rightarrow> (
+        (('pt \<rightharpoonup> 'v discr \<times> 'perm) \<times> fail_st) \<times> ('x \<Rightarrow> 'v) \<Rightarrow>
+        (('pt \<rightharpoonup> 'v discr \<times> 'perm) \<times> fail_st) \<times> ('x \<Rightarrow> 'v) \<Rightarrow>
+        bool)\<close>
+  where
+    \<open>heap_read_rel x pt \<equiv>
+      \<lambda>((l,fl),s) ((l',fl'),s').
+        (\<exists>v \<pi>. l pt = Some (v, \<pi>) \<and> l' = l \<and> s' = s(x := the_discr v) \<and> fl' = Running) \<or>
+        (l pt = None \<or> fl = Failed) \<and> l' = l \<and> s' = s \<and> fl' = Failed\<close>
+
+abbreviation \<open>HeapRead x pt \<equiv> \<langle> heap_read_rel x pt \<rangle>\<close>
+lemmas HeapRead_def = heap_read_rel_def
+
+
+lemma rgsat_heap_read:
+  fixes p :: \<open>('x \<Rightarrow> 'v) \<Rightarrow> bool\<close>
+    and x v R \<pi> pt
+  defines \<open>heap_read_guar \<equiv> (\<lambda>s s'. s' = s(x := v))\<close>
+  and \<open>precond \<equiv> pt \<^bold>\<mapsto>\<^bsub>\<pi>\<^esub> (\<lambda>_. v) \<sqinter> wssa R (\<S> (\<lambda>s. p (s(x := v))))\<close>
+  and \<open>postcond \<equiv> pt \<^bold>\<mapsto>\<^bsub>\<pi>\<^esub> (\<lambda>_. v) \<sqinter> sswa R (\<S> p)\<close>
 assumes
-    \<open>rel_image snd ra_ptr_read \<le> G\<close>
+    \<open>heap_read_guar \<le> G\<close>
     \<open>precond \<le> I\<close>
     \<open>postcond \<le> I\<close>
     \<open>T RGSepAtom\<close>
   shows
-    \<open>R, G, I, F, T \<turnstile>\<^sub>f { precond } PointerRead x pt { postcond }\<close>
+    \<open>R, G, I, F, T \<turnstile>\<^sub>f { precond } HeapRead x pt { postcond }\<close>
   using assms
-  unfolding PointerRead_def
 proof (intro rgsat_atom[where p=\<open>nofailure_pred precond\<close> and q=\<open>nofailure_pred postcond\<close>])
-  let ?ra' = \<open>step_fail_lift (\<lambda>(l, s) (l', s', fl').
-               case l pt of None \<Rightarrow>
-                  l' = l \<and> s' = s \<and> fl' = Failed
-               | Some (v, xa) \<Rightarrow>
-                  l' = l \<and> s' = s(x := the_discr v) \<and> fl' = Running)\<close>
-
-  show \<open>nofailure_pred precond \<le> wssa (R \<times>\<^sub>R (=)) (nofailure_pred precond)\<close>
+  show \<open>nofailure_pred precond \<le> wssa R (nofailure_pred precond)\<close>
     unfolding precond_def
-    by (simp add: wlp_inf)
+    by (clarsimp simp add: wlp_def points_to_perm_def, meson rtranclp_trans)
+  then show \<open>sswa R (nofailure_pred precond) \<le> nofailure_pred I\<close>
+    using assms(5)
+    by (meson order_trans subpred_pred_times_eq_res_ppABC_to_ppACB_iff wlp_weaker_iff_sp_stronger)
 
-  show \<open>sswa (R \<times>\<^sub>R (=)) (nofailure_pred postcond) \<le> nofailure_pred postcond\<close>
+  show \<open>sswa R (nofailure_pred postcond) \<le> nofailure_pred postcond\<close>
     unfolding postcond_def
-    by simp
-
-  show \<open>\<forall>f\<le>nofailure_pred F. sp ?ra' (nofailure_pred precond \<^emph>\<and> f) \<le> nofailure_pred postcond \<^emph>\<and> any_shared f\<close>
-    unfolding any_shared_def ra_ptr_read_def precond_def postcond_def
-    apply (clarsimp simp add: sp_step_fail_lift_on_nofailure_pred_eq subset_nofailure_pred_iff
-        predTimes3_sepconj_conj_distrib[symmetric] case_option_disj_iff)
-    apply (clarsimp simp add: sepconj_conj_def points_to_def plus_option_iff)
-    apply (metis (mono_tags, lifting) Discr_inverse_iff comp_apply snd_conv sswa_trivial wssa_trivial)
-    done
+    by (clarsimp simp add: sp_def points_to_perm_def, meson rtranclp_trans)
+  then show \<open>sswa R (nofailure_pred postcond) \<le> nofailure_pred I\<close>
+    using assms(6)
+    by (meson order_trans subpred_pred_times_eq_res_ppABC_to_ppACB_iff wlp_weaker_iff_sp_stronger)
 
   show
-    \<open>rel_image snd
-      (rel_liftL (nofailure_pred precond \<^emph>\<and> nofailure_pred F) \<sqinter> ?ra')
-    \<le> G \<times>\<^sub>R (=)\<close>
-    using assms(4)
-    apply (simp only: predTimes3_sepconj_conj_distrib[symmetric] predTimes3_sup_distrib[symmetric])
-    apply (unfold ra_ptr_read_def precond_def postcond_def)
-    apply (clarsimp simp add: sepconj_conj_def points_to_def plus_option_iff rel_image_def
-        le_fun_def ex_disj_distrib all_conj_distrib split: option.splits)
-    apply (force simp add: wlp_def plus_option_iff ex_disj_distrib all_conj_distrib)
+    \<open>\<forall>f\<le>nofailure_pred F. sp (heap_read_rel x pt) (nofailure_pred precond \<^emph>\<and> f) \<le>
+      nofailure_pred postcond \<^emph>\<and> any_shared f\<close>
+    unfolding any_shared_def precond_def postcond_def
+    apply (simp add: all_subpred_pred_times_eq_res_ppABC_to_ppACB_internalise)
+    apply (clarsimp simp add: sp_def points_to_perm_def sepconj_conj_def heap_read_rel_def)
+    apply (clarsimp simp add: plus_option_def split: option.splits)
+     apply (metis (mono_tags) comp_apply not_dom_then_singleton_plus_heap_eq wssa_trivial
+        rtranclp.rtrancl_refl snd_conv)
+    apply (metis (mono_tags) comp_apply rtranclp.rtrancl_refl snd_conv wssa_trivial)
     done
+
+  show \<open>rel_image snd (rel_liftL (nofailure_pred precond \<^emph>\<and> nofailure_pred F) \<sqinter> heap_read_rel x pt)
+          \<le> G\<close>
+    using assms(4)
+    unfolding heap_read_guar_def precond_def
+    by (force simp add: heap_read_rel_def sepconj_conj_def plus_option_iff points_to_perm_def)
 qed simp+
 
 
-section \<open> PointerWrite \<close>
+subsection \<open> Heap Write \<close>
 
-definition PointerWrite
-  :: \<open>'pt \<Rightarrow> ('s \<Rightarrow> 'v) \<Rightarrow> (('pt \<rightharpoonup> 'v discr \<times> 'perm) \<times> ('s \<times> fail_st)) comm\<close>
+definition heap_write_rel
+  :: \<open>'pt \<Rightarrow> ('s \<Rightarrow> 'v) \<Rightarrow> ((('pt \<rightharpoonup> 'v discr \<times> 'perm) \<times> fail_st) \<times> 's) \<Rightarrow> _ \<Rightarrow> bool\<close>
   where
-    \<open>PointerWrite pt e \<equiv>
-      Atomic (step_fail_lift (\<lambda>(l, s) (l', s', fl').
-        case l pt of
-          Some (_, perm) \<Rightarrow> l' = l(pt \<mapsto> (Discr (e s), perm)) \<and> s' = s \<and> fl' = Running
-        | None \<Rightarrow> l' = l \<and> s' = s \<and> fl' = Failed
-      ))\<close>
+    \<open>heap_write_rel pt e \<equiv>
+      \<lambda>((l,fl),s) ((l',fl'),s').
+        s' = s \<and> (
+          (\<exists>v perm. l pt = Some (v, perm) \<and> fl = Running \<and> l' = l(pt \<mapsto> (Discr (e s), perm)) \<and> fl' = Running) \<or>
+          (l pt = None \<or> fl = Failed) \<and> l' = l \<and> fl' = Failed)\<close>
+
+abbreviation \<open>HeapWrite pt e \<equiv> \<langle> heap_write_rel pt e \<rangle>\<close>
+
+
+lemma heap_write_rel_nofailure_rel_eq:
+  \<open>sp (heap_write_rel pt e) (nofailure_pred p) =
+    nofailure_pred (
+      sp
+        (\<lambda>(l,s) (l',s'). s' = s \<and> (\<exists>v perm. l pt = Some (v, perm) \<and> l' = l(pt \<mapsto> (Discr (e s), perm))))
+        p)
+    \<squnion> failure_pred ((\<lambda>(l',s'). l' pt = None) \<sqinter> p)\<close>
+  apply (clarsimp simp add: heap_write_rel_def sp_def fun_eq_iff split: prod.splits)
+  apply (case_tac b, force)
+  apply clarsimp
+  apply (metis (no_types, lifting) ext)
+  done
+
+lemma rgsat_pointer_write:
+  fixes e pt p R \<pi> v
+  defines \<open>precond \<equiv> (pt \<^bold>\<mapsto>\<^bsub>\<pi>\<^esub> (\<lambda>_. v)) \<sqinter> wssa R (\<S> p)\<close>
+    and \<open>postcond \<equiv> sswa R (pt \<^bold>\<mapsto>\<^bsub>\<pi>\<^esub> e \<sqinter> \<S> p)\<close>
+  assumes
+    \<comment> \<open> this is the side condition that constrains permissions to be exclusive \<close>
+    \<open>F \<le> - \<L> (\<Squnion>x'\<in>Collect ((##) (Discr v, \<pi>)). pt \<^bold>\<mapsto>\<^sup>\<Up> x')\<close>
+    \<open>(=) \<le> G\<close>
+    \<open>precond \<le> I\<close>
+    \<open>postcond \<le> I\<close>
+    \<open>T RGSepAtom\<close>
+  shows
+    \<open>R, G, I, F, T \<turnstile>\<^sub>f { precond } HeapWrite pt e { postcond }\<close>
+  using assms
+proof (intro rgsat_atom[where p=\<open>nofailure_pred precond\<close> and q=\<open>nofailure_pred postcond\<close>])
+  show \<open>nofailure_pred precond \<le> wssa R (nofailure_pred precond)\<close>
+    unfolding precond_def
+    by (clarsimp simp add: points_to_perm_def wlp_def, meson rtranclp_trans)
+  then show \<open>sswa R (nofailure_pred precond) \<le> nofailure_pred I\<close>
+    by (meson assms(5) nofailure_pred_strong_mono order_trans wlp_weaker_iff_sp_stronger)
+
+  show \<open>sswa R (nofailure_pred postcond) \<le> nofailure_pred postcond\<close>
+    unfolding postcond_def
+    by (clarsimp simp add: points_to_perm_def sp_def, metis rtranclp_trans)
+  then show \<open>sswa R (nofailure_pred postcond) \<le> nofailure_pred I\<close>
+    using assms(6) by fastforce
+
+  have failure_helper: \<open>\<And>f. failure_pred ((\<lambda>(l', s'). l' pt = None) \<sqinter> (precond \<^emph>\<and> f)) = \<bottom>\<close>
+    by (clarsimp simp add: fun_eq_iff precond_def points_to_perm_def sepconj_conj_def
+        plus_option_iff, blast)
+
+  let ?ra = \<open>(\<lambda>(l, s) (l', s'). s' = s \<and> (\<exists>v perm. l pt = Some (v, perm) \<and> l' = l(pt \<mapsto> (Discr (e s), perm))))\<close>
+  let ?frame2 =
+    \<open>\<forall>f\<le>F. sp ?ra (precond \<^emph>\<and> f) \<le> postcond \<^emph>\<and> any_shared f\<close>
+  let ?frame1 =
+    \<open>\<forall>f\<le>nofailure_pred F.
+      sp (heap_write_rel pt e) (nofailure_pred precond \<^emph>\<and> f) \<le>
+        nofailure_pred postcond \<^emph>\<and> any_shared f\<close>
+
+  have \<open>\<top> = ?frame2\<close>
+    using assms(3)
+    unfolding precond_def postcond_def
+    apply (clarsimp simp add: sp_def le_fun_def points_to_perm_def points_to_upcl_def
+        sepconj_conj_def plus_option_iff)
+    apply (elim disjE)
+      (* None case *)
+     apply clarsimp
+     apply (rename_tac s l)
+     apply (rule_tac x=\<open>[pt \<mapsto> (Discr (e s), \<pi>)]\<close> in exI)
+     apply (rule_tac x=l in exI)
+     apply (intro conjI)
+        apply fastforce
+       apply fastforce
+      apply fastforce
+     apply fastforce
+      (* Some case, prevented by frame exclusivity *)
+    apply clarsimp
+    apply (rename_tac ss ls fs v' \<pi>')
+    apply (subgoal_tac \<open>v' = Discr v\<close>)
+     prefer 2
+     apply (simp add: disjoint_fun_def disjoint_option_def split: option.splits)
+     apply metis
+    apply (subgoal_tac \<open>\<pi> ## \<pi>'\<close>)
+     prefer 2
+     apply clarsimp
+     apply (metis disjoint_fun_def disjoint_option_simps(1) disjoint_prod_def fun_upd_same snd_conv)
+    apply blast
+    done
+  also have \<open>... = ?frame1\<close>
+    by (simp add: all_subpred_pred_times_eq_res_ppABC_to_ppACB_internalise failure_helper
+        nofailure_pred_sepconj_conj_distrib[symmetric] heap_write_rel_nofailure_rel_eq
+        any_shared_pred_times_eq_res_ppABC_to_ppACB_distrib)
+  finally show ?frame1
+    by simp
+
+  show
+    \<open>rel_image snd (rel_liftL (nofailure_pred precond \<^emph>\<and> nofailure_pred F) \<sqinter> heap_write_rel pt e) \<le>
+      G\<close>
+    using assms(4)
+    by (clarsimp simp add: heap_write_rel_def nofailure_pred_sepconj_conj_distrib[symmetric]
+        le_fun_def)
+qed simp+
 
 lemma top_write_frame_cond_iff_all_disjoint_perm:
   \<open>\<top> \<le> - \<L> (\<Squnion>x'\<in>Collect ((##) (Discr v, \<pi>)). pt \<^bold>\<mapsto>\<^sup>\<Up> x') \<longleftrightarrow> (\<forall>\<pi>'. \<not> \<pi> ## \<pi>')\<close>
   by (force simp add: points_to_upcl_def le_fun_def)
 
-lemma nofailure_pred_any_shared_semidistrib:
-  \<open>nofailure_pred (any_shared p) \<le> any_shared (nofailure_pred p)\<close>
-  by (simp add: nofailure_pred_def any_shared_def le_fun_def)
 
-lemma rgsat_pointer_write:
-  fixes e pt p R \<pi> v
-  defines \<open>ra_ptr_write \<equiv> (\<lambda>(l,s) (l',s'). l' = l(pt \<mapsto> e s) \<and> s' = s)\<close>
-    and \<open>precond \<equiv> \<L> (pt \<^bold>\<mapsto>\<^bsub>\<pi>\<^esub> v) \<sqinter> wssa R (\<S> p)\<close>
-    and \<open>postcond \<equiv> sswa R ((\<lambda>(ls, ss). (pt \<^bold>\<mapsto>\<^bsub>\<pi>\<^esub> (e ss)) ls) \<sqinter> \<S> p)\<close>
+subsection \<open> Heap Alloc \<close>
+
+definition heap_alloc_rel
+  :: \<open>('s \<Rightarrow> 'v) \<Rightarrow> ((('pt \<rightharpoonup> 'v discr \<times> 'perm::pre_perm_alg) \<times> fail_st) \<times> 's) \<Rightarrow> _ \<Rightarrow> bool\<close>
+  where
+    \<open>heap_alloc_rel e \<equiv>
+      \<lambda>((l,fl),s) ((l',fl'),s').
+        s' = s \<and> (
+          (\<exists>pt \<pi>. l pt = None \<and> (\<forall>\<pi>'. \<not> \<pi> ## \<pi>') \<and> l' = l(pt \<mapsto> (Discr (e s), \<pi>))) \<and>
+            fl = Running \<and> fl' = fl \<or>
+          (fl = Failed \<or> (\<forall>pt. l pt \<noteq> None) \<or> (\<forall>\<pi>::'perm. \<exists>\<pi>'. \<pi> ## \<pi>')) \<and> l' = l \<and> fl' = Failed
+      )\<close>
+
+abbreviation \<open>HeapAlloc e \<equiv> \<langle> heap_alloc_rel e \<rangle>\<close>
+
+
+lemma rgsat_pointer_alloc:
+  fixes p pt e R
+  defines \<open>precond \<equiv> \<L> emp \<sqinter> wssa R (\<S> p)\<close>
+  \<comment> \<open> we obtain a is \<^emph>\<open>some\<close> totally disjoint permission \<close>
+  and \<open>postcond \<equiv> (\<Squnion>pt. \<Squnion>\<pi>1\<in>{\<pi>1::'perm::pre_perm_alg. \<forall>\<pi>. \<not> \<pi>1 ## \<pi>}. sswa R (pt \<^bold>\<mapsto>\<^bsub>\<pi>1\<^esub> e \<sqinter> \<S> p))\<close>
   assumes
-    \<comment> \<open> this is the side condition that constrains permissions to be exclusive \<close>
-    \<open>F \<le> - \<L> (\<Squnion>x'\<in>Collect ((##) (Discr v, \<pi>)). pt \<^bold>\<mapsto>\<^sup>\<Up> x')\<close>
-    \<open>rel_image snd ra_ptr_write \<le> G\<close>
+    \<open>(=) \<le> G\<close>
     \<open>precond \<le> I\<close>
     \<open>postcond \<le> I\<close>
     \<open>T RGSepAtom\<close>
+    and frame_not_maximal_heap: \<open>F \<le> - (\<L> maximal_heap)\<close>
+    and maximal_perm_ex: \<open>\<exists>\<pi>::'perm. \<forall>\<pi>'. \<not> \<pi> ## \<pi>'\<close>
   shows
-    \<open>R, G, I, F, T \<turnstile>\<^sub>f { precond } PointerWrite pt e { postcond }\<close>
+    \<open>R, G, I, F, T \<turnstile>\<^sub>f { precond } HeapAlloc e { postcond }\<close>
   using assms
-  unfolding PointerWrite_def
 proof (intro rgsat_atom[where p=\<open>nofailure_pred precond\<close> and q=\<open>nofailure_pred postcond\<close>])
-  let ?ra' = \<open>step_fail_lift (\<lambda>(l, s) (l', s', fl').
-                case l pt of
-                  None \<Rightarrow> l' = l \<and> s' = s \<and> fl' = Failed
-                | Some (x, perm) \<Rightarrow> l' = l(pt \<mapsto> (Discr (e s), perm)) \<and> s' = s \<and> fl' = Running)\<close>
-
-  show \<open>nofailure_pred precond \<le> wssa (R \<times>\<^sub>R (=)) (nofailure_pred precond)\<close>
+  show \<open>nofailure_pred precond \<le> wssa R (nofailure_pred precond)\<close>
     unfolding precond_def
-    apply (clarsimp simp add: points_to_def wlp_def)
-    apply (metis rtranclp_trans)
-    done
-
-  show \<open>sswa (R \<times>\<^sub>R (=)) (nofailure_pred postcond) \<le> nofailure_pred postcond\<close>
-    unfolding postcond_def
-    apply (clarsimp simp add: fun_eq_iff le_fun_def points_to_def sp_def)
-    apply (metis rtranclp_trans)
-    done
-
-  let ?frame5 =
-    \<open>(\<forall>f\<le>F. \<forall>lf s'.
-      f (lf, s') \<longrightarrow>
-      [pt \<mapsto> (Discr v, \<pi>)] ## lf \<longrightarrow>
-      R\<^sup>*\<^sup>* s' \<le> p \<longrightarrow>
-      (\<exists>s. R\<^sup>*\<^sup>* s s' \<and> p s \<and>
-        [pt \<mapsto> (Discr (e s), \<pi>)] ## lf \<and>
-        Some (Discr (e s'), \<pi>) + lf pt = Some (Discr (e s), \<pi>) + lf pt))\<close>
-  let ?frame4 =
-    \<open>(\<forall>f\<le>F. \<forall>lf s'.
-      f (lf, s') \<longrightarrow>
-      [pt \<mapsto> (Discr v, \<pi>)] ## lf \<longrightarrow>
-      R\<^sup>*\<^sup>* s' \<le> p \<longrightarrow>
-      (\<exists>s. R\<^sup>*\<^sup>* s s' \<and> p s \<and>
-        [pt \<mapsto> (Discr (e s), \<pi>)] ## lf \<and>
-        [pt \<mapsto> (Discr (e s'), \<pi>)] + lf = [pt \<mapsto> (Discr (e s), \<pi>)] + lf))\<close>
-  let ?frame3 =
-    \<open>(\<forall>f\<le>F. \<forall>l' s'.
-       (\<exists>lx.
-          [pt \<mapsto> (Discr v, \<pi>)] ## lx \<and>
-          l' = [pt \<mapsto> (Discr (e s'), \<pi>)] + lx \<and>
-          (\<forall>b. R\<^sup>*\<^sup>* s' b \<longrightarrow> p b) \<and>
-          f (lx, s')) \<longrightarrow>
-       (\<exists>lx s.
-          [pt \<mapsto> (Discr (e s), \<pi>)] ## lx \<and>
-          l' = [pt \<mapsto> (Discr (e s), \<pi>)] + lx \<and>
-          R\<^sup>*\<^sup>* s s' \<and>
-          p s \<and>
-          (\<exists>ss. f (lx, ss))))\<close>
-  let ?frame2 =
-    \<open>(\<forall>f\<le>F. \<forall>l \<pi> s.
-      l pt = None \<longrightarrow>
-      (\<exists>v. (precond \<^emph>\<and> f) (l(pt \<mapsto> (Discr v, \<pi>)), s)) \<longrightarrow>
-      (postcond \<^emph>\<and> any_shared f) (l(pt \<mapsto> (Discr (e s), \<pi>)), s))\<close>
-  let ?frame1 =
-    \<open>\<forall>f\<le>nofailure_pred F.
-      sp ?ra' (nofailure_pred precond \<^emph>\<and> f) \<le> nofailure_pred postcond \<^emph>\<and> any_shared f\<close>
-
-
-  have \<open>?frame5 = ?frame4\<close>
-    apply (clarsimp simp add: le_fun_def points_to_upcl_def)
-    sorry
-
-  have \<open>\<top> = ?frame4\<close>
+    by (clarsimp simp add: wlp_def emp_def, meson rtranclp_trans)
+  then show \<open>sswa R (nofailure_pred precond) \<le> nofailure_pred I\<close>
     using assms(4)
-    apply (clarsimp simp add: le_fun_def points_to_upcl_def)
-    sorry
-  also have \<open>... = ?frame3\<close>
-    apply (rule iffI)
-     apply (metis predicate1I)
-    apply clarsimp
-    apply (drule_tac x=\<open>(=) (lf, s')\<close> in spec)
-    apply blast
-    done
-  also have \<open>... = ?frame2\<close>
-    unfolding precond_def postcond_def points_to_def
-    apply (clarsimp simp add: fun_eq_iff sepconj_conj_def plus_option_iff all_conj_distrib
-        any_shared_def sp_def wlp_def split: if_splits)
-    apply (intro iff_allI imp_cong[OF refl])
-    sorry
-(*
-    apply (rule imp_cong)
-      (* assm equiv *)
-     apply (simp add: disjoint_fun_def disjoint_option_def option_ex_split plus_option_iff2)
-     apply (rule iffI)
-      (** \<Rightarrow> *)
-      apply clarsimp
-      apply (elim exE disjE conjE; simp?) (* +1 *)
-      (*** \<open>pt\<close> in the frame *)
-       apply (rename_tac \<pi>')
-       apply (rule_tac x=\<open>lx(pt \<mapsto> (Discr v, \<pi> + \<pi>'))\<close> in exI)
-       apply simp
-       apply (rule_tac x=\<open>[pt \<mapsto> (Discr v, \<pi>)]\<close> in exI)
-       apply (rule_tac x=lx in exI)
-       apply force
-      (*** \<open>pt\<close> not in frame *)
-      apply (rule_tac x=\<open>lx(pt \<mapsto> (Discr v, \<pi>))\<close> in exI)
-      apply simp
-      apply (rule_tac x=\<open>[pt \<mapsto> (Discr v, \<pi>)]\<close> in exI)
-      apply (rule_tac x=lx in exI)
+    by (meson nofailure_pred_strong_mono order.trans wlp_weaker_iff_sp_stronger)
+
+  show \<open>sswa R (nofailure_pred postcond) \<le> nofailure_pred postcond\<close>
+    unfolding postcond_def
+    by (clarsimp simp add: points_to_perm_def sp_def heap_upd_eq_iff, metis rtranclp_trans)
+  then show \<open>sswa R (nofailure_pred postcond) \<le> nofailure_pred I\<close>
+    using assms(5) nofailure_pred_strong_mono by blast
+
+  show \<open>\<forall>f\<le>nofailure_pred F. sp (heap_alloc_rel e) (nofailure_pred precond \<^emph>\<and> f) \<le> nofailure_pred postcond \<^emph>\<and> any_shared f\<close>
+    unfolding precond_def postcond_def
+    apply (simp add: all_subpred_pred_times_eq_res_ppABC_to_ppACB_internalise
+        nofailure_pred_sepconj_conj_distrib[symmetric]
+        any_shared_pred_times_eq_res_ppABC_to_ppACB_distrib)
+    apply (clarsimp simp add: heap_alloc_rel_def sp_def wlp_def emp_def le_fun_def sepconj_conj_def)
+    apply (rename_tac ls fl ss fs)
+    apply (elim disjE conjE)
+      apply (clarsimp simp add: points_to_perm_def)
+      apply (simp add: ex_simps[symmetric] del: ex_simps)
+      apply (rule_tac x=fs in exI)
+      apply (rule_tac x=ss in exI)
+      apply (rule_tac x=pt in exI)
+      apply (rule_tac x=\<pi> in exI)
+      apply (rule_tac x=ss in exI)
       apply force
-      (** \<Leftarrow> *)
-     apply (clarsimp simp add: plus_option_iff)
-     apply (erule disjE)
-      apply (metis plus_option_simps(3))
-     apply clarsimp
-     apply (rename_tac hf dv \<pi>')
-     apply (rule_tac x=hf in exI)
-     apply clarsimp
-     apply (metis option.inject option.simps(3) prod.inject)
-      (* conseq equiv *)
-    apply (clarsimp simp add: disjoint_fun_def disjoint_option_def
-        plus_option_iff plus_option_iff2 disj.assoc[symmetric])
-    apply (subst option_ex_split)
-    apply (simp split: option.splits)
-    apply (rename_tac la lb)
-    apply (rule iffI)
-      (** \<Rightarrow> *)
-     apply clarsimp
-     apply (rename_tac lf s ss)
-     apply (rule_tac x=\<open>[pt \<mapsto> (Discr (e s), \<pi>)]\<close> in exI)
-     apply (rule_tac x=lf in exI)
-     apply (intro conjI)
-        apply (clarsimp; fail)
-       apply (clarsimp simp add: plus_option_iff2; fail)
-      apply (rule_tac x=\<open>[pt \<mapsto> (Discr (e s), \<pi>)]\<close> in exI)
-      apply (simp, blast)
-     apply blast
-      (** \<Leftarrow> *)
-    apply (clarsimp simp add: plus_option_iff)
-    apply (elim disjE; metis (no_types))
-    done
-*)
-  also have \<open>... = ?frame1\<close>
-    apply -
-    apply (simp add: all_impl_nofailure_pred_internalise sp_step_fail_lift_on_nofailure_pred_eq
-        predTimes3_sepconj_conj_distrib[symmetric])
-    apply (simp add: option_ex_split nofailure_pred_def le_fun_def ex_disj_distrib
-        conj_disj_distribR sepconj_conj_def)
-    apply (intro iffI)
-     apply clarsimp
-     apply (rule conjI)
-      apply (clarsimp simp add: precond_def points_to_def sepconj_conj_def plus_option_iff)
-
-    sorry
-  finally show ?frame1
-    by simp
-
-  show
-    \<open>rel_image snd
-      (rel_liftL (nofailure_pred precond \<^emph>\<and> nofailure_pred F) \<sqinter> ?ra')
-    \<le> G \<times>\<^sub>R (=)\<close>
-    using assms(5)
-    apply (simp only: predTimes3_sepconj_conj_distrib[symmetric] predTimes3_sup_distrib[symmetric])
-    apply (unfold ra_ptr_write_def precond_def postcond_def)
-    apply (clarsimp simp add: sepconj_conj_def points_to_def plus_option_iff rel_image_def
-        le_fun_def ex_disj_distrib all_conj_distrib split: option.splits)
+      (* contradiction between maximal frame and no maximal frame assumption. *)
+     apply (cut_tac frame_not_maximal_heap)
+     apply (clarsimp simp add: Sup_fun_def sepconj_conj_def ex_simps(1-4)[symmetric]
+        emp_def le_fun_def maximal_heap_def simp del: ex_simps(1-4))
+     apply (metis not_Some_prod_eq)
+      (* contradiction between no maximal perm and maximal_perm_ex assumption. *)
+    apply (cut_tac maximal_perm_ex)
     apply force
     done
+
+  show \<open>rel_image snd (rel_liftL (nofailure_pred precond \<^emph>\<and> nofailure_pred F) \<sqinter> heap_alloc_rel e) \<le> G\<close>
+    using assms(3)
+    by (fastforce simp add: heap_alloc_rel_def)
 qed simp+
+
+
+subsection \<open> Heap Free \<close>
+
+definition heap_free_rel
+  :: \<open>'pt \<Rightarrow> ((('pt \<rightharpoonup> 'v discr \<times> 'perm::pre_perm_alg) \<times> fail_st) \<times> 's) \<Rightarrow> _ \<Rightarrow> bool\<close>
+  where
+    \<open>heap_free_rel pt \<equiv>
+      (\<lambda>(l,fl) (l',fl').
+        (\<exists>x. l pt = Some x \<and> l' = l(pt := None)) \<and> fl = Running \<and> fl' = fl \<or>
+        (fl = Failed \<or> l pt = None) \<and> l' = l \<and> fl' = Failed
+      ) \<times>\<^sub>R (=)\<close>
+
+abbreviation \<open>HeapFree pt \<equiv> \<langle> heap_free_rel pt \<rangle>\<close>
+
+
+lemma rgsat_heap_free:
+  fixes pt e R p
+    and \<pi> :: \<open>'perm :: pre_perm_alg\<close>
+  defines \<open>precond \<equiv> wssa R (pt \<^bold>\<mapsto>\<^bsub>\<pi>\<^esub> e \<sqinter> \<S> p)\<close>
+    and \<open>postcond \<equiv> \<L> emp \<sqinter> sswa R (\<S> p)\<close>
+  assumes
+    \<open>(=) \<le> G\<close>
+    \<open>precond \<le> I\<close>
+    \<open>postcond \<le> I\<close>
+    \<open>T RGSepAtom\<close>
+    and frames_disjoint_at_pt:
+    \<open>F \<le> - \<L>\<^sub>S (\<lambda>ss. (\<Squnion>x'\<in>Collect ((##) (Discr (e ss), \<pi>)). pt \<^bold>\<mapsto>\<^sup>\<Up> x'))\<close>
+  shows
+    \<open>R, G, I, F, T \<turnstile>\<^sub>f { precond } HeapFree pt { postcond }\<close>
+  using assms
+proof (intro rgsat_atom[where p=\<open>nofailure_pred precond\<close> and q=\<open>nofailure_pred postcond\<close>])
+  show \<open>nofailure_pred precond \<le> wssa R (nofailure_pred precond)\<close>
+    unfolding precond_def
+    by (clarsimp simp add: wlp_def, metis rtranclp_trans)
+  then show \<open>sswa R (nofailure_pred precond) \<le> nofailure_pred I\<close>
+    using assms(4)
+    by (meson nofailure_pred_strong_mono order.trans wlp_weaker_iff_sp_stronger)
+
+  show \<open>sswa R (nofailure_pred postcond) \<le> nofailure_pred postcond\<close>
+    unfolding postcond_def
+    by (clarsimp simp add: points_to_perm_def  emp_def sp_def heap_upd_eq_iff, metis rtranclp_trans)
+  then show \<open>sswa R (nofailure_pred postcond) \<le> nofailure_pred I\<close>
+    using assms(5) nofailure_pred_strong_mono by blast
+
+  show \<open>\<forall>f\<le>nofailure_pred F.
+          sp (heap_free_rel pt) (nofailure_pred precond \<^emph>\<and> f) \<le>
+            nofailure_pred postcond \<^emph>\<and> any_shared f\<close>
+    unfolding precond_def postcond_def heap_free_rel_def emp_def
+    apply (simp add: all_subpred_pred_times_eq_res_ppABC_to_ppACB_internalise
+        nofailure_pred_sepconj_conj_distrib[symmetric]
+        any_shared_pred_times_eq_res_ppABC_to_ppACB_distrib)
+    apply (clarsimp simp add: sp_def wlp_def points_to_perm_def sepconj_conj_def plus_option_iff)
+    apply (rename_tac lfs fl ss ls fs)
+      \<comment> \<open> Replacing \<open>x\<close> with \<open>(e ss)\<close> here causes simplifier loops. Presumably because
+            the stabilised predicate we are deriving this from can now show many \<open>e ss = e ss'\<close>
+            lemmas. \<close>
+    apply (subgoal_tac \<open>\<exists>x. ls = [pt \<mapsto> (Discr x, \<pi>)]\<close>)
+     prefer 2
+     apply force
+    apply clarsimp
+    apply (rule conjI, force)
+    apply (elim disjE)
+     apply clarsimp
+     apply (metis fun_upd_triv)
+      (* find a contradiction with the disjoint frame assm *)
+    apply (cut_tac frames_disjoint_at_pt)
+    apply (clarsimp simp add: disjoint_fun_def disjoint_option_def points_to_upcl_def le_fun_def
+        split: if_splits)
+    apply (metis (mono_tags, lifting) fst_conv heap_upd_eq_iff rtranclp.rtrancl_refl)
+    done
+
+  show \<open>rel_image snd (rel_liftL (nofailure_pred precond \<^emph>\<and> nofailure_pred F) \<sqinter> heap_free_rel pt) \<le> G\<close>
+    using assms(3)
+    by (fastforce simp add: heap_free_rel_def)
+qed simp+
+
 
 end
